Design a better spec format for parsers.

examples/sampler/verif_sampler_ingress_parser.v
@@ -7,6 +7,7 @@ Require Import ProD3.examples.sampler.ModelRepr.
 Require Import ProD3.examples.sampler.common.
 Require Import ProD3.examples.sampler.verif_sampler_tofino_parser.
 Require Import ProD3.core.ProgNotations.
+Require Import ProD3.core.PacketFormat.
 Require Import Poulet4.P4light.Syntax.P4Notations.
 Require Import Hammer.Plugin.Hammer.
 Require Export Coq.Program.Program.
@@ -22,8 +23,8 @@ Definition parser_parse_udp_spec: func_spec :=
     PATH p
     MOD (Some [["hdr"]]) [["packet_in"]]
     WITH (pin: packet_in) hdr udp pin'
-         (_: extract udp_h pin =
-             Some (udp, SReturnNull, pin')),
+         (_: ⊫ᵥ udp \: udp_h)
+         (_: pin ⫢ [⦑ encode udp ⦒; ⦑ pin' ⦒]),
       PRE
         (ARG []
         (MEM [(["hdr"], hdr)]
@@ -37,7 +38,11 @@ Lemma parser_parse_udp_body:
   func_sound ge parser_parse_udp_fundef nil parser_parse_udp_spec.
 Proof.
   start_function.
-  step_call (@packet_in_extract_body Info); [ entailer | apply H |].
+  simpl_format_list.
+  step_call (@packet_in_extract_body Info);
+    [ entailer | apply extract_encode; [assumption | reflexivity] |].
+  simpl_format_list.
+  apply format_match_nil in H2. subst p0. rewrite app_nil_r.
   step_call (@parser_accept_body Info). entailer.
   step. entailer.
 Qed.
@@ -50,8 +55,8 @@ Definition parser_parse_tcp_spec: func_spec :=
     PATH p
     MOD (Some [["hdr"]]) [["packet_in"]]
     WITH (pin: packet_in) hdr tcp pin'
-         (_: extract tcp_h pin =
-             Some (tcp, SReturnNull, pin')),
+         (_: ⊫ᵥ tcp \: tcp_h)
+         (_: pin ⫢ [⦑ encode tcp ⦒; ⦑ pin' ⦒]),
       PRE
         (ARG []
         (MEM [(["hdr"], hdr)]
@@ -65,7 +70,10 @@ Lemma parser_parse_tcp_body:
   func_sound ge parser_parse_tcp_fundef nil parser_parse_tcp_spec.
 Proof.
   start_function.
-  step_call (@packet_in_extract_body Info); [ entailer | apply H |].
+  simpl_format_list.
+  step_call (@packet_in_extract_body Info);
+    [ entailer | apply extract_encode; [assumption | reflexivity] |].
+  do 2 simpl_format_list. rewrite app_nil_r.
   step_call (@parser_accept_body Info). entailer.
   step. entailer.
 Qed.
@@ -106,20 +114,16 @@ Definition ipv4_repr_val (ipv4: ipv4_rec): Val :=
      ("src_addr", ipv4_src_addr ipv4);
      ("dst_addr", ipv4_dst_addr ipv4)] true.
 
-Definition protocol_extract_cond
-  (ipv4: ipv4_rec) (pin pin': packet_in) (result: Val): Prop :=
-  if Val_eqb (ipv4_protocol ipv4) (P4BitV 8 IP_PROTOCOLS_TCP)
-  then extract tcp_h pin = Some (result, SReturnNull, pin')
-  else if Val_eqb (ipv4_protocol ipv4) (P4BitV 8 IP_PROTOCOLS_UDP)
-       then extract udp_h pin = Some (result, SReturnNull, pin')
-       else result = ValBaseNull /\ pin = pin'.
+Definition is_tcp ipv4: bool :=
+  Val_eqb (ipv4_protocol ipv4) (P4BitV 8 IP_PROTOCOLS_TCP).
+
+Definition is_udp ipv4: bool :=
+  Val_eqb (ipv4_protocol ipv4) (P4BitV 8 IP_PROTOCOLS_UDP).
 
 Definition protocol_extract_result
   (ipv4: ipv4_rec) (result: Val) (header: Sval): Sval :=
-  if Val_eqb (ipv4_protocol ipv4) (P4BitV 8 IP_PROTOCOLS_TCP)
-  then update "tcp" (eval_val_to_sval result) header
-  else if Val_eqb (ipv4_protocol ipv4) (P4BitV 8 IP_PROTOCOLS_UDP)
-       then update "udp" (eval_val_to_sval result) header
+  if is_tcp ipv4 then update "tcp" (eval_val_to_sval result) header
+  else if is_udp ipv4 then update "udp" (eval_val_to_sval result) header
        else header.
 
 Record header_sample_rec := {
@@ -144,10 +148,14 @@ Definition parser_parse_ipv4_spec: func_spec :=
   WITH,
     PATH p
     MOD (Some [["hdr"]]) [["packet_in"]]
-    WITH (pin: packet_in) hsample ipv4 pin2 result pin3
-         (_: extract ipv4_h pin =
-               Some (ipv4_repr_val ipv4, SReturnNull, pin2))
-         (_: protocol_extract_cond ipv4 pin2 pin3 result),
+    WITH (pin: packet_in) hsample ipv4 result pin'
+         (_: ⊫ᵥ ipv4_repr_val ipv4 \: ipv4_h)
+         (_: if is_tcp ipv4 then ⊫ᵥ result \: tcp_h
+             else if is_udp ipv4 then ⊫ᵥ result \: udp_h
+                  else result = ValBaseNull)
+         (_: pin ⫢ [ ⦑ encode (ipv4_repr_val ipv4) ⦒;
+                     ⦃ is_tcp ipv4 ? ⦑ encode result ⦒ |
+                       ⦃ is_udp ipv4 ? ⦑ encode result ⦒ | ε ⦄ ⦄; ⦑ pin' ⦒] ),
       PRE
         (ARG []
         (MEM [(["hdr"], (hdr hsample))]
@@ -157,7 +165,7 @@ Definition parser_parse_ipv4_spec: func_spec :=
            (MEM [(["hdr"], protocol_extract_result ipv4 result
                              (update "ipv4" (eval_val_to_sval (ipv4_repr_val ipv4))
                                 (hdr hsample)))]
-           (EXT [ExtPred.singleton ["packet_in"] (ObjPin pin3)]))).
+           (EXT [ExtPred.singleton ["packet_in"] (ObjPin pin')]))).
 
 Lemma force_cast_P4BitV_eq: forall w v,
     force ValBaseNull (@Ops.eval_cast Info (TypBit w) (P4BitV w v)) = P4BitV w v.
@@ -215,20 +223,27 @@ Lemma parser_parse_ipv4_body:
   func_sound ge parser_parse_ipv4_fundef nil parser_parse_ipv4_spec.
 Proof.
   start_function.
-  step_call (@packet_in_extract_body Info); [ entailer | apply H |].
+  simpl_format_list.
+  step_call (@packet_in_extract_body Info);
+    [ entailer | apply extract_encode; [assumption | reflexivity] |].
   step_if; change (ValBaseBit _) with (P4BitV 8 IP_PROTOCOLS_TCP) in H1;
     rewrite abs_ipv4_hdr_eq_eq in H1.
-  - apply is_sval_true_binary_op_eq in H1. red in H0. rewrite H1 in H0.
-    unfold protocol_extract_result. rewrite !H1.
-    step_call parser_parse_tcp_body. 2: apply H0. entailer.
-  - apply is_sval_false_binary_op_eq in H1. red in H0. rewrite H1 in H0.
-    unfold protocol_extract_result. rewrite !H1.
+  - apply is_sval_true_binary_op_eq in H1.
+    change (Val_eqb _ _) with (is_tcp ipv4) in H1. unfold protocol_extract_result.
+    rewrite H1 in *. simpl_format_list.
+    step_call parser_parse_tcp_body; [ entailer | assumption | apply H3 ].
+  - apply is_sval_false_binary_op_eq in H1.
+    change (Val_eqb _ _) with (is_tcp ipv4) in H1.
+    unfold protocol_extract_result. rewrite H1 in *. simpl_format_list.
     step_if; change (ValBaseBit _) with (P4BitV 8 IP_PROTOCOLS_UDP) in H2;
       rewrite abs_ipv4_hdr_eq_eq in H2.
-    + apply is_sval_true_binary_op_eq in H2. rewrite H2 in H0.
-      rewrite !H2. step_call parser_parse_udp_body. 2: apply H0. entailer.
-    + apply is_sval_false_binary_op_eq in H2. rewrite H2 in H0.
-      destruct H0. subst. rewrite !H2.
+    + apply is_sval_true_binary_op_eq in H2.
+      change (Val_eqb _ _) with (is_udp ipv4) in H2.
+      rewrite H2 in *. simpl_format_list.
+      step_call parser_parse_udp_body; [ entailer | assumption | apply H3 ].
+    + apply is_sval_false_binary_op_eq in H2.
+      change (Val_eqb _ _) with (is_udp ipv4) in H2.
+      rewrite H2 in *. do 4 simpl_format_list. rewrite app_nil_r.
       step_call (@parser_accept_body Info). entailer.
 Qed.
 
@@ -261,12 +276,16 @@ Definition parser_parse_ethernet_spec: func_spec :=
   WITH,
     PATH p
     MOD (Some [["hdr"]]) [["packet_in"]]
-    WITH (pin pin2 pin3 pin4: packet_in) ether ipv4 hsample result
-         (_: extract ethernet_h pin =
-               Some (ethernet_repr_val ether, SReturnNull, pin2))
-         (_: extract ipv4_h pin2 =
-               Some (ipv4_repr_val ipv4, SReturnNull, pin3))
-         (_: protocol_extract_cond ipv4 pin3 pin4 result)
+    WITH (pin pin': packet_in) ether ipv4 hsample result
+         (_: ⊫ᵥ ethernet_repr_val ether \: ethernet_h)
+         (_: ⊫ᵥ ipv4_repr_val ipv4 \: ipv4_h)
+         (_: if is_tcp ipv4 then ⊫ᵥ result \: tcp_h
+             else if is_udp ipv4 then ⊫ᵥ result \: udp_h
+                  else result = ValBaseNull)
+         (_: pin ⫢ [ ⦑ encode (ethernet_repr_val ether) ⦒;
+                     ⦑ encode (ipv4_repr_val ipv4) ⦒;
+                     ⦃ is_tcp ipv4 ? ⦑ encode result ⦒ |
+                       ⦃ is_udp ipv4 ? ⦑ encode result ⦒ | ε ⦄ ⦄; ⦑ pin' ⦒] )
          (_: ethernet_ether_type ether = P4BitV 16 ETHERTYPE_IPV4),
       PRE
         (ARG []
@@ -275,7 +294,7 @@ Definition parser_parse_ethernet_spec: func_spec :=
       POST
         (ARG_RET [] ValBaseNull
            (MEM [(["hdr"], ethernet_extract_result hsample ether ipv4 result)]
-              (EXT [ExtPred.singleton ["packet_in"] (ObjPin pin4)]))).
+              (EXT [ExtPred.singleton ["packet_in"] (ObjPin pin')]))).
 
 Lemma abs_ether_eq_eq: forall ether hsample w v,
     abs_eq
@@ -299,9 +318,11 @@ Lemma parser_parse_ethernet_body:
   func_sound ge parser_parse_ethernet_fundef nil parser_parse_ethernet_spec.
 Proof.
   start_function.
-  step_call (@packet_in_extract_body Info); [ entailer | apply H |].
-  step_if; change (ValBaseBit _) with (P4BitV 16 ETHERTYPE_IPV4) in H3;
-    rewrite abs_ether_eq_eq in H3.
+  simpl_format_list.
+  step_call (@packet_in_extract_body Info);
+    [ entailer | apply extract_encode; [assumption | reflexivity] |].
+  step_if; change (ValBaseBit _) with (P4BitV 16 ETHERTYPE_IPV4) in H2;
+    rewrite abs_ether_eq_eq in H2.
   - unfold ethernet_extract_result.
     remember (Build_header_sample_rec
                 (header_sample_bridge hsample)
@@ -313,9 +334,9 @@ Proof.
     assert (update "ethernet" (eval_val_to_sval (ethernet_repr_val ether))
               (hdr hsample) = hdr new_hdr) by (rewrite Heqnew_hdr; reflexivity).
     rewrite H4.
-    step_call parser_parse_ipv4_body; [entailer| apply H0 | apply H1].
-  - apply is_sval_false_binary_op_eq in H3.
-    rewrite Val_eqb_neq_iff in H3. exfalso. apply H3. assumption.
+    step_call parser_parse_ipv4_body; [entailer | apply H0 | apply H1 | apply H5].
+  - apply is_sval_false_binary_op_eq in H2.
+    rewrite Val_eqb_neq_iff in H2. exfalso. apply H2. assumption.
 Qed.
 
 Definition parser_start_fundef :=
@@ -345,16 +366,19 @@ Definition parser_start_spec: func_spec :=
   WITH,
     PATH p
     MOD (Some [["hdr"]; ["ig_intr_md"]]) [["packet_in"]]
-    WITH (pin pin2 pin3 pin4 pin5: packet_in) ver port stamp
-         ether ipv4 hsample has_sample result
-         (_: extract ingress_intrinsic_metadata_t pin =
-             Some (iimt_repr_val 0 ver port stamp, SReturnNull, pin2))
-         (_: 64 < Zlength pin2)
-         (_: extract ethernet_h (skipn 64 pin2) =
-               Some (ethernet_repr_val ether, SReturnNull, pin3))
-         (_: extract ipv4_h pin3 =
-               Some (ipv4_repr_val ipv4, SReturnNull, pin4))
-         (_: protocol_extract_cond ipv4 pin4 pin5 result)
+    WITH (pin pin': packet_in) ver port stamp ether ipv4 hsample has_sample result
+         (_: ⊫ᵥ iimt_repr_val 0 ver port stamp \: ingress_intrinsic_metadata_t)
+         (_: ⊫ᵥ ethernet_repr_val ether \: ethernet_h)
+         (_: ⊫ᵥ ipv4_repr_val ipv4 \: ipv4_h)
+         (_: if is_tcp ipv4 then ⊫ᵥ result \: tcp_h
+             else if is_udp ipv4 then ⊫ᵥ result \: udp_h
+                  else result = ValBaseNull)
+         (_: pin ⫢ [⦑ encode (iimt_repr_val 0 ver port stamp) ⦒;
+                    ⟨64⟩;
+                    ⦑ encode (ethernet_repr_val ether) ⦒;
+                     ⦑ encode (ipv4_repr_val ipv4) ⦒;
+                     ⦃ is_tcp ipv4 ? ⦑ encode result ⦒ |
+                       ⦃ is_udp ipv4 ? ⦑ encode result ⦒ | ε ⦄ ⦄; ⦑ pin' ⦒] )
          (_: ethernet_ether_type ether = P4BitV 16 ETHERTYPE_IPV4),
       PRE
         (ARG []
@@ -366,13 +390,26 @@ Definition parser_start_spec: func_spec :=
                              ((sample_valid_bridge hsample has_sample))
                              ether ipv4 result);
                  (["ig_intr_md"], (iimt_repr_sval 0 ver port stamp))]
-              (EXT [ExtPred.singleton ["packet_in"] (ObjPin pin5)]))).
+              (EXT [ExtPred.singleton ["packet_in"] (ObjPin pin')]))).
 
 Lemma parser_start_body:
   func_sound ge parser_start_fundef nil parser_start_spec.
 Proof.
   start_function.
-  step_call tofino_parser_body; [entailer | eauto.. |].
+  change [⦑ encode (iimt_repr_val 0 ver port stamp) ⦒;
+          ⟨ 64 ⟩; ⦑ encode (ethernet_repr_val ether) ⦒;
+          ⦑ encode (ipv4_repr_val ipv4) ⦒;
+          ⦃ is_tcp ipv4 ? ⦑ encode result ⦒
+          | ⦃ is_udp ipv4 ? ⦑ encode result ⦒ | ε ⦄ ⦄;
+          ⦑ pin' ⦒] with
+    ([⦑ encode (iimt_repr_val 0 ver port stamp) ⦒; ⟨ 64 ⟩] ++
+       [⦑ encode (ethernet_repr_val ether) ⦒;
+        ⦑ encode (ipv4_repr_val ipv4) ⦒;
+        ⦃ is_tcp ipv4 ? ⦑ encode result ⦒
+        | ⦃ is_udp ipv4 ? ⦑ encode result ⦒ | ε ⦄ ⦄;
+        ⦑ pin' ⦒]) in H3. rewrite format_match_app_iff' in H3.
+  destruct H3 as [p1 [p2 [? [? ?]]]].
+  step_call tofino_parser_body; [ entailer | apply H | apply H5 | ].
   step. simpl eval_write_var.
   change (ValBaseStruct _) with (hdr (sample_valid_bridge hsample has_sample)).
   step_call parser_parse_ethernet_body;
@@ -437,16 +474,19 @@ Definition parser_spec: func_spec :=
   WITH,
     PATH p
     MOD (Some [["hdr"]; ["ig_md"]; ["ig_intr_md"]]) [["packet_in"]]
-    WITH (pin pin2 pin3 pin4 pin5: packet_in) ver port stamp
-         ether ipv4 result
-         (_: extract ingress_intrinsic_metadata_t pin =
-             Some (iimt_repr_val 0 ver port stamp, SReturnNull, pin2))
-         (_: 64 < Zlength pin2)
-         (_: extract ethernet_h (skipn 64 pin2) =
-               Some (ethernet_repr_val ether, SReturnNull, pin3))
-         (_: extract ipv4_h pin3 =
-               Some (ipv4_repr_val ipv4, SReturnNull, pin4))
-         (_: protocol_extract_cond ipv4 pin4 pin5 result)
+    WITH (pin pin': packet_in) ver port stamp ether ipv4 result
+         (_: ⊫ᵥ iimt_repr_val 0 ver port stamp \: ingress_intrinsic_metadata_t)
+         (_: ⊫ᵥ ethernet_repr_val ether \: ethernet_h)
+         (_: ⊫ᵥ ipv4_repr_val ipv4 \: ipv4_h)
+         (_: if is_tcp ipv4 then ⊫ᵥ result \: tcp_h
+             else if is_udp ipv4 then ⊫ᵥ result \: udp_h
+                  else result = ValBaseNull)
+         (_: pin ⫢ [⦑ encode (iimt_repr_val 0 ver port stamp) ⦒;
+                    ⟨64⟩;
+                    ⦑ encode (ethernet_repr_val ether) ⦒;
+                     ⦑ encode (ipv4_repr_val ipv4) ⦒;
+                     ⦃ is_tcp ipv4 ? ⦑ encode result ⦒ |
+                       ⦃ is_udp ipv4 ? ⦑ encode result ⦒ | ε ⦄ ⦄; ⦑ pin' ⦒] )
          (_: ethernet_ether_type ether = P4BitV 16 ETHERTYPE_IPV4),
       PRE
         (ARG []
@@ -459,7 +499,7 @@ Definition parser_spec: func_spec :=
                   (ValBaseStruct [("num_pkts", P4Bit_ 32)]);
                   (iimt_repr_sval 0 ver port stamp)] ValBaseNull
            (MEM []
-              (EXT [ExtPred.singleton ["packet_in"] (ObjPin pin5)]))).
+              (EXT [ExtPred.singleton ["packet_in"] (ObjPin pin')]))).
 
 Lemma parser_body:
   func_sound ge parser_fundef nil parser_spec.
