core/PacketFormat.v
@@ -1,0 +1,271 @@
+Require Import Poulet4.P4light.Syntax.P4defs.
+Require Import Poulet4.P4light.Architecture.Tofino.
+Require Import Poulet4.P4light.Semantics.Typing.ValueTyping.
+
+Notation packet := (list bool).
+
+Section PacketFormat.
+
+  Context {tags_t: Type}.
+  Notation Val := (@ValueBase bool).
+  Notation P4Type := (@P4Type tags_t).
+
+  Fixpoint encode (val: Val): packet :=
+    match val with
+    | ValBaseBool b => [b]
+    | ValBaseBit bit => bit
+    | ValBaseInt bit => bit
+    | ValBaseTuple l => concat (map encode l)
+    | ValBaseStruct vs => concat (map (fun '(_, v) => encode v) vs)
+    | ValBaseHeader fields true => concat (map (fun '(_, v) => encode v) fields)
+    | _ => []
+    end.
+
+  Fixpoint is_packet_typ (typ: P4Type) : bool :=
+    match typ with
+    | TypBool
+    | TypBit _
+    | TypInt _ => true
+    | TypTuple l => forallb is_packet_typ l
+    | TypHeader flds
+    | TypStruct flds => AList.key_unique flds &&
+                         forallb (is_packet_typ ∘ snd) flds
+    | _ => false
+    end.
+
+  Fixpoint header_is_valid (val: Val) : bool :=
+    match val with
+    | ValBaseHeader _ false => false
+    | ValBaseStruct fields
+    | ValBaseHeader fields true => forallb (header_is_valid ∘ snd) fields
+    | ValBaseTuple l => forallb header_is_valid l
+    | _ => true
+    end.
+
+  Ltac auto_unfold :=
+    repeat match goal with
+    | [ |- context [Packet.packet_bind]] => unfold Packet.packet_bind
+    | [ |- context [Packet.packet_ret]] => unfold Packet.packet_ret
+    | [ |- context [ExceptionState.state_bind]] => unfold ExceptionState.state_bind
+    | [ |- context [ExceptionState.state_return]] =>
+        unfold ExceptionState.state_return
+      end.
+
+  Ltac simpl_more :=
+    repeat match goal with
+      | H: _ && _ = true |- _ => rewrite andb_true_iff in H; destruct H
+      | H: forallb header_is_valid (_ :: _) = true |- _ => simpl in H
+      | H: is_packet_typ (TypTuple (_ :: _)) = true |- _ => simpl in H
+      | H: is_packet_typ (TypStruct _) = true |- _ => simpl in H
+      | H: is_packet_typ (TypHeader _) = true |- _ => simpl in H
+      | H1: ?P, H2: ?P -> _ |- _ => specialize (H2 H1); clear H1
+      | H: _ /\ _ |- _ => destruct H
+      | H: (if ?b then _ else false) = true |- _ => destruct b; [|discriminate]
+      end.
+
+  Lemma extract_bits_app: forall bits pkt,
+      Packet.extract_bits (length bits) (bits ++ pkt) = (inl bits, pkt).
+  Proof.
+    intros. unfold Packet.extract_bits. simpl.
+    auto_unfold. unfold Packet.verify, Packet.pkt_min_size.
+    cut ((length bits <=? length (bits ++ pkt))%nat = true).
+    - intros. rewrite H. simpl. rewrite firstn_app2, skipn_app2 by lia.
+      rewrite Nat.sub_diag, app_nil_r. reflexivity.
+    - rewrite Nat.leb_le, app_length. lia.
+  Qed.
+
+  Definition ext_val_typ (val: Val) (typ: P4Type): Prop :=
+    ⊢ᵥ val \: typ /\ header_is_valid val = true.
+
+  Lemma extract_encode_raw: forall (typ: P4Type) (val: Val) pkt,
+      ext_val_typ val typ  ->
+      is_packet_typ typ = true ->
+      Extract.extract typ (encode val ++ pkt) = (inl val, pkt).
+  Proof.
+    intros ? ? ? [] ?. revert pkt.
+    induction H using custom_val_typ_ind; simpl in H0;
+      try discriminate; intros; simpl; rewrite ?Nat2N.id; auto_unfold;
+      rewrite ?extract_bits_app; try reflexivity.
+    - induction H; simpl; auto. auto_unfold. inv H2. simpl_more.
+      rewrite <- app_assoc, H7.
+      remember (sequence (map Extract.extract l') (concat (map encode l) ++ pkt)).
+      destruct p, s; inversion IHForall2. reflexivity.
+    - simpl_more. clear H H1. remember (clear_AList_tags ts) as cs.
+      revert dependent ts.
+      induction H2; intros; destruct ts as [|[k v] ts]; try discriminate; auto.
+      simpl in *. auto_unfold. inv Heqcs. inv H3. simpl_more.
+      destruct x. simpl in *. subst s. clear H4. rewrite <- app_assoc, H5.
+      specialize (IHForall2 ts ltac:(reflexivity) H3). clear H3 H5.
+      remember (asequence (map (fun '(k, v) => (str k, Extract.extract v)) ts)
+                  (concat (map (fun '(_, v) => encode v) l) ++ pkt)).
+      destruct p, s; inversion IHForall2. reflexivity.
+    - simpl_more. clear H H1. remember (clear_AList_tags ts) as cs.
+      revert dependent ts.
+      induction H2; intros; destruct ts as [|[k v] ts];
+        try discriminate; simpl_more; auto.
+      simpl in *. auto_unfold. inv Heqcs. inv H3. simpl_more.
+      destruct x. simpl in *. subst s. clear H5. rewrite <- app_assoc, H6.
+      specialize (IHForall2 ts ltac:(reflexivity) H4). clear H4 H6.
+      remember (asequence (map (fun '(k, v) => (str k, Extract.extract v)) ts)
+                  (concat (map (fun '(_, v) => encode v) l) ++ pkt)).
+      destruct p, s; inversion IHForall2. reflexivity.
+  Qed.
+
+  Lemma extract_encode: forall (typ: P4Type) (val: Val) pkt,
+      ext_val_typ val typ  ->
+      is_packet_typ typ = true ->
+      extract typ (encode val ++ pkt) = Some (val, SReturnNull, pkt).
+  Proof. intros. unfold extract. rewrite extract_encode_raw; auto. Qed.
+
+End PacketFormat.
+
+Inductive format :=
+| null: format
+| accurate: packet -> format
+| unspecified: nat -> format
+| guarded: bool -> format -> format -> format.
+
+Inductive match_one: format -> packet -> Prop :=
+| match_null: match_one null []
+| match_accurate: forall p, match_one (accurate p) p
+| match_unspecified: forall p n, length p = n -> match_one (unspecified n) p
+| match_guarded_true: forall p f1 f2,
+    match_one f1 p -> match_one (guarded true f1 f2) p
+| match_guarded_false: forall p f1 f2,
+    match_one f2 p -> match_one (guarded false f1 f2) p.
+
+Lemma match_one_accurate: forall a p, match_one (accurate a) p -> a = p.
+Proof. intros. inversion H. reflexivity. Qed.
+
+Lemma match_one_guarded_true: forall p f1 f2,
+    match_one (guarded true f1 f2) p -> match_one f1 p.
+Proof. intros. inversion H. assumption. Qed.
+
+Lemma match_one_guarded_false: forall p f1 f2,
+    match_one (guarded false f1 f2) p -> match_one f2 p.
+Proof. intros. inversion H. assumption. Qed.
+
+
+Lemma match_one_size_eq: forall f p1 p2,
+    match_one f p1 -> match_one f p2 -> length p1 = length p2.
+Proof. induction f; intros; inv H; inv H0; auto. Qed.
+
+Definition format_match (f: list format) (p: packet): Prop :=
+  exists l, concat l = p /\ Forall2 match_one f l.
+
+Lemma format_match_size: forall p n f,
+    format_match (unspecified n :: f) p -> (Z.of_nat n) <= Zlength p.
+Proof.
+  intros. destruct H as [l [? ?]]. destruct l; inv H0. inv H4.
+  simpl. rewrite Zlength_app, <- Zlength_correct.
+  pose proof (Zlength_nonneg (concat l0)). lia.
+Qed.
+
+Lemma format_match_skipn: forall p n p',
+    format_match [unspecified n ; accurate p'] p -> skipn n p = p'.
+Proof.
+  intros. destruct H as [l [? ?]]. inv H0. inv H5. inv H4. inv H3. inv H1.
+  simpl. rewrite app_nil_r, skipn_app, skipn_all, Nat.sub_diag. reflexivity.
+Qed.
+
+Lemma format_match_cons_iff: forall f l p,
+    format_match (f :: l) p <->
+      exists p1 p2,  p = p1 ++ p2 /\ match_one f p1 /\ format_match l p2.
+Proof.
+  intros. split; intros.
+  - inv H. destruct H0. inv H0. simpl. exists y, (concat l').
+    split; [|split]; auto. exists l'. split; auto.
+  - destruct H as [p1 [p2 [? [? [pl []]]]]].
+    exists (p1 :: pl). split; simpl; [rewrite H1 | constructor]; auto.
+Qed.
+
+Lemma format_match_nil: forall p, format_match [] p -> p = [].
+Proof. intros. destruct H as [l []]. inv H0. reflexivity. Qed.
+
+Lemma format_match_guarded_true: forall f1 f2 l p,
+    format_match (guarded true f1 f2 :: l) p -> format_match (f1 :: l) p.
+Proof.
+  intros. rewrite format_match_cons_iff in H. destruct H as [p1 [p2 [? [? ?]]]].
+  apply match_one_guarded_true in H0. rewrite format_match_cons_iff.
+  exists p1, p2. split; auto.
+Qed.
+
+Lemma format_match_guarded_false: forall f1 f2 l p,
+    format_match (guarded false f1 f2 :: l) p -> format_match (f2 :: l) p.
+Proof.
+  intros. rewrite format_match_cons_iff in H. destruct H as [p1 [p2 [? [? ?]]]].
+  apply match_one_guarded_false in H0. rewrite format_match_cons_iff.
+  exists p1, p2. split; auto.
+Qed.
+
+Lemma format_match_null: forall l p,
+    format_match (null :: l) p -> format_match l p.
+Proof.
+  intros. rewrite format_match_cons_iff in H. destruct H as [p1 [p2 [? [? ?]]]].
+  inversion H0. subst p1. simpl in H. subst p2. assumption.
+Qed.
+
+Ltac simpl_format_list :=
+  match goal with
+  | H: format_match (accurate _ :: _) ?p |- _ =>
+      rewrite format_match_cons_iff in H;
+      let p1 := fresh "p1" in
+      let p2 := fresh "p2" in
+      destruct H as [p1 [p2 [? [? ?]]]]; subst p;
+      match goal with
+      | HS: match_one (accurate _) ?ps |- _ =>
+          apply match_one_accurate in HS; subst ps
+      end
+  | H: format_match (guarded true _ _ :: _) _ |- _ =>
+      apply format_match_guarded_true in H
+  | H: format_match (guarded false _ _ :: _) _ |- _ =>
+      apply format_match_guarded_false in H
+  | H: format_match (null :: _) _ |- _ =>
+      apply format_match_null in H
+  | H: format_match nil ?p |- _ =>
+      apply format_match_nil in H; subst p
+  end.
+
+Lemma format_match_app_iff: forall l1 l2 p,
+    format_match (l1 ++ l2) p <->
+      exists p1 p2,  p = p1 ++ p2 /\ format_match l1 p1 /\ format_match l2 p2.
+Proof.
+  induction l1; intros; simpl.
+  - split; intros.
+    + exists nil, p. simpl. split; [|split]; auto. exists nil. simpl. split; auto.
+    + destruct H as [p1 [p2 [? [? ?]]]]. destruct H0 as [l1 [? ?]].
+      inv H2. simpl. assumption.
+  - rewrite format_match_cons_iff.
+    split; intros; destruct H as [p1 [p2 [? [? ?]]]]; subst.
+    + rewrite IHl1 in H1. destruct H1 as [p3 [p4 [? [? ?]]]]. subst p2.
+      exists (p1 ++ p3), p4. split; [|split]; auto. 1: rewrite app_assoc; reflexivity.
+      rewrite format_match_cons_iff. exists p1, p3. split; auto.
+    + rewrite format_match_cons_iff in H0. destruct H0 as [p3 [p4 [? [? ?]]]].
+      subst. rewrite <- app_assoc. exists p3, (p4 ++ p2). split; [|split]; auto.
+      rewrite IHl1. exists p4, p2. split; auto.
+Qed.
+
+Lemma format_match_app_iff': forall l1 l2 p,
+    format_match (l1 ++ l2) p <->
+      exists p1 p2,  p = p1 ++ p2 /\
+                  format_match (l1 ++ [accurate p2]) p /\
+                  format_match l2 p2.
+Proof.
+  intros. split; intros.
+  - rewrite format_match_app_iff in H. destruct H as [p1 [p2 [? [? ?]]]]; subst.
+    exists p1, p2. split; [|split]; auto. rewrite format_match_app_iff.
+    exists p1, p2. split; [|split]; auto. exists [p2]. simpl. rewrite app_nil_r. split; auto.
+    repeat constructor.
+  - destruct H as [p1 [p2 [? [? ?]]]]; subst. rewrite format_match_app_iff.
+    exists p1, p2. split; [|split]; auto. rewrite format_match_app_iff in H0.
+    destruct H0 as [p3 [p4 [? [? ?]]]]. inv H2. destruct H3. inv H3. inv H8.
+    inv H6. simpl in H. rewrite app_nil_r in H. apply app_inv_tail in H.
+    subst. assumption.
+Qed.
+
+Notation "'ε'" := (null).
+Notation "⦑ p ⦒" := (accurate p).
+Notation "⟨ n ⟩" := (unspecified n).
+Notation "⦃ b ? f1 | f2 ⦄" := (guarded b f1 f2).
+Notation "p ⫢ f" := (format_match f p) (at level 80, no associativity).
+Notation "'⊫ᵥ' v '\:' t" := (ext_val_typ v t) (at level 80, no associativity).
